revm: more simulations for helper functions of calls

RocqOfRust/revm/revm_interpreter/instructions/contract/simulate/call_helpers.v
@@ -1,16 +1,25 @@
 Require Import simulate.RocqOfRust.
 Require Import alloy_primitives.bytes.links.mod.
+Require Import alloy_primitives.bytes.simulate.mod.
 Require Import alloy_primitives.links.aliases.
+Require Import core.links.array.
 Require Import core.num.simulate.mod.
 Require Import core.ops.links.range.
+Require Import core.ops.simulate.deref.
+Require Import core.ops.simulate.range.
 Require Import revm.revm_context_interface.links.journaled_state.
+Require Import revm.revm_interpreter.gas.simulate.calc.
 Require Import revm.revm_interpreter.instructions.contract.links.call_helpers.
 Require Import revm.revm_interpreter.instructions.simulate.macros.
+Require Import revm.revm_interpreter.interpreter.simulate.shared_memory.
 Require Import revm.revm_interpreter.links.gas.
 Require Import revm.revm_interpreter.links.interpreter.
 Require Import revm.revm_interpreter.links.interpreter_types.
 Require Import revm.revm_interpreter.simulate.gas.
 Require Import revm.revm_interpreter.simulate.interpreter_types.
+Require Import revm.revm_specification.links.hardfork.
+Require Import revm.revm_specification.simulate.hardfork.
+Require Import ruint.simulate.lib.
 
 Definition resize_memory
     {WIRE : Set} `{Link WIRE}
@@ -24,9 +33,10 @@ Definition resize_memory
     (fun len interpreter =>
   if len.(Integer.value) =? 0 then
     let offset := Impl_usize.MAX in
-    ( Some {|
+    (
+      Some {|
         Range.start := offset;
-        Range.end_ := {| Integer.value := offset.(Integer.value) + len.(Integer.value) |}
+        Range.end_ := offset +i len;
       |},
       interpreter
     )
@@ -34,15 +44,16 @@ Definition resize_memory
     as_usize_or_fail_ret_macro interpreter offset None
       (fun interpreter => (None, interpreter))
       (fun offset interpreter =>
-        resize_memory_macro interpreter offset len
-          (fun interpreter => (None, interpreter))
-          (fun interpreter =>
-            ( Some {|
-                Range.start := offset;
-                Range.end_ := {| Integer.value := offset.(Integer.value) + len.(Integer.value) |}
-              |},
-              interpreter
-            )))).
+    resize_memory_macro interpreter offset len
+      (fun interpreter => (None, interpreter))
+      (fun interpreter =>
+    (
+      Some {|
+        Range.start := offset;
+        Range.end_ := offset +i len;
+      |},
+      interpreter
+    )))).
 
 Lemma resize_memory_eq
     {WIRE : Set} `{Link WIRE}
@@ -55,28 +66,106 @@ Lemma resize_memory_eq
     (offset len : aliases.U256.t)
     (stack : Stack.t) :
   let ref_interpreter := make_ref 0 in
-  let result_interpreter := resize_memory interpreter offset len in
+  let result := resize_memory interpreter offset len in
   {{
     SimulateM.eval_f (
       run_resize_memory run_InterpreterTypes_for_WIRE ref_interpreter offset len
     )
     (interpreter :: stack)%stack 🌲
     (
-      Output.Success (fst result_interpreter),
-      (snd result_interpreter :: stack)%stack
+      Output.Success (fst result),
+      (snd result :: stack)%stack
     )
   }}.
 Proof.
+  apply Run.remove_extra_stack1.
+  with_strategy transparent [run_resize_memory] unfold run_resize_memory; cbn.
+  unfold resize_memory.
+  lu. c. {
+    apply Impl_Uint.as_limbs_eq; repeat unshelve econstructor.
+  }
+  lu. cw Impl_usize.max_eq.
+  repeat cp.
+  destruct Bool.eqb eqn:?; r. {
+    lu. cw InterpreterTypesEq.
+    admit.
+  }
+  lu. repeat cp.
+  destruct Bool.eqb eqn:? in |-*; r.
+  { lu. c. {
+      apply Impl_Uint.as_limbs_eq; repeat unshelve econstructor.
+    }
+    lu. cw Impl_usize.max_eq.
+    repeat cp.
+    destruct Bool.eqb eqn:? in |-*; r. {
+      lu. cw InterpreterTypesEq.
+      admit.
+    }
+    (* resize_memory! *)
+    lu.
+    cw Impl_usize.saturating_add_eq.
+    cw num_words_eq.
+    lu.
+    cw InterpreterTypesEq.
+    cw @Impl_Gas.record_memory_expansion_eq.
+    l. {
+      cp.
+      cw InterpreterTypesEq.
+      p.
+    }
+    cp.
+    pf.
+    all: admit.
+  }
+  { c. {
+      apply Impl_usize.max_eq.
+    }
+    cp.
+    pf.
+    all: admit.
+  }
 Admitted.
 
-
-Parameter get_memory_input_and_out_ranges :
-  forall
+Definition get_memory_input_and_out_ranges
     {WIRE : Set} `{Link WIRE}
-    {WIRE_types : InterpreterTypes.Types.t} `{InterpreterTypes.Types.AreLinks WIRE_types},
-  Interpreter.t WIRE WIRE_types ->
-  option (Bytes.t * Range.t usize) *
-  Interpreter.t WIRE WIRE_types.
+    {WIRE_types : InterpreterTypes.Types.t} `{InterpreterTypes.Types.AreLinks WIRE_types}
+    {IInterpreterTypes : InterpreterTypes.C WIRE_types}
+    (interpreter : Interpreter.t WIRE WIRE_types) :
+    option (Bytes.t * Range.t usize) * Interpreter.t WIRE WIRE_types :=
+  popn_macro interpreter {| Integer.value := 4 |}
+    (fun interpreter => (None, interpreter))
+    (fun arr interpreter =>
+  let '⟬ in_offset; in_len; out_offset; out_len ⟭ := arr.(array.value) in
+
+  let '(in_range_opt, interpreter) := resize_memory interpreter in_offset in_len in
+  match in_range_opt with
+  | None => (None, interpreter)
+  | Some in_range =>
+
+  let input :=
+    if Impl_Range.is_empty in_range then
+      Impl_Bytes.new
+    else
+      let slice :=
+        IInterpreterTypes.(InterpreterTypes.MemoryTrait_for_Memory).(MemoryTrait.slice)
+            interpreter.(Interpreter.memory)
+            in_range in
+      let slice : list u8 :=
+        IInterpreterTypes
+          .(InterpreterTypes.MemoryTrait_for_Memory)
+          .(MemoryTrait.Deref_for_Synthetic)
+          .(Deref.deref)
+          .(RefStub.projection)
+          slice in
+      Impl_Bytes.copy_from_slice slice in
+
+  let '(ret_range_opt, interpreter) := resize_memory interpreter out_offset out_len in
+  match ret_range_opt with
+  | None => (None, interpreter)
+  | Some ret_range =>
+  (Some (input, ret_range), interpreter)
+
+  end end).
 
 Lemma get_memory_input_and_out_ranges_eq
     {WIRE : Set} `{Link WIRE}
@@ -101,43 +190,53 @@ Lemma get_memory_input_and_out_ranges_eq
   }}.
 Proof.
   apply Run.remove_extra_stack1.
-  with_strategy transparent [run_get_memory_input_and_out_ranges] unfold run_get_memory_input_and_out_ranges; cbn.
-  idtac.
-  unfold popn_macro;
-  eapply Run.Call; [
-    apply InterpreterTypesEq
-      .(InterpreterTypes.Eq.StackTrait_for_Stack)
-      .(StackTrait.Eq.popn)
-  |];
-  destruct _.(InterpreterTypes.StackTrait_for_Stack).(StackTrait.popn) as [[|] ?]; cbn; [|
-    apply Run.LetUnfold;
-    cbn;
-    eapply Run.Call; [
-      apply InterpreterTypesEq
-        .(InterpreterTypes.Eq.LoopControl_for_Control)
-        .(LoopControl.Eq.set_instruction_result)
-    |];
-    cbn
-  ].
-  2: {
-    admit.
-  }
+  with_strategy transparent [run_get_memory_input_and_out_ranges]
+    unfold run_get_memory_input_and_out_ranges, get_memory_input_and_out_ranges;
+    cbn.
+  popn_macro_eq InterpreterTypesEq.
+  lu.
+  cw @resize_memory_eq.
 Admitted.
 
-Parameter calc_call_gas :
-  forall
+Definition calc_call_gas
     {WIRE : Set} `{Link WIRE}
-    {WIRE_types : InterpreterTypes.Types.t} `{InterpreterTypes.Types.AreLinks WIRE_types},
-  Interpreter.t WIRE WIRE_types ->
-  AccountLoad.t ->
-  bool ->
-  u64 ->
-  option u64 * Interpreter.t WIRE WIRE_types.
+    {WIRE_types : InterpreterTypes.Types.t} `{InterpreterTypes.Types.AreLinks WIRE_types}
+    {IInterpreterTypes : InterpreterTypes.C WIRE_types}
+    {IRuntimeFlag : RuntimeFlag.C WIRE_types.(InterpreterTypes.Types.RuntimeFlag)}
+    (interpreter : Interpreter.t WIRE WIRE_types)
+    (account_load : AccountLoad.t)
+    (has_transfer : bool)
+    (local_gas_limit : u64) :
+    option u64 * Interpreter.t WIRE WIRE_types :=
+  let spec_id := IRuntimeFlag.(RuntimeFlag.spec_id) interpreter.(Interpreter.runtime_flag) in
+  let call_cost := call_cost spec_id has_transfer account_load in
+  gas_macro interpreter call_cost
+    (fun interpreter => (None, interpreter))
+    (fun interpreter =>
+
+  let gas_limit :=
+    if Impl_SpecId.is_enabled_in spec_id SpecId.TANGERINE then
+      let gas :=
+        IInterpreterTypes
+          .(InterpreterTypes.LoopControl_for_Control)
+          .(LoopControl.gas)
+          .(RefStub.projection)
+          interpreter.(Interpreter.control) in
+      let remaining := Impl_Gas.remaining_63_of_64_parts gas in
+      Z.min i[remaining] i[local_gas_limit] : u64
+    else
+      local_gas_limit in
+
+  (Some gas_limit, interpreter)
+  ).
 
 Lemma calc_call_gas_eq
     {WIRE : Set} `{Link WIRE}
     {WIRE_types : InterpreterTypes.Types.t} `{InterpreterTypes.Types.AreLinks WIRE_types}
     (run_InterpreterTypes_for_WIRE : InterpreterTypes.Run WIRE WIRE_types)
+    `{IInterpreterTypes : !InterpreterTypes.C WIRE_types}
+    `{InterpreterTypesEq :
+      !InterpreterTypes.Eq.t WIRE WIRE_types run_InterpreterTypes_for_WIRE IInterpreterTypes}
     (interpreter : Interpreter.t WIRE WIRE_types)
     (account_load : AccountLoad.t)
     (has_transfer : bool)
