RocqOfRust/alloy_primitives/bytes/simulate/mod.v
@@ -1,0 +1,38 @@
+Require Import simulate.RocqOfRust.
+Require Import alloy_primitives.bytes.links.mod.
+
+Module Impl_Bytes.
+  Definition Self : Set :=
+    Bytes.t.
+
+  Definition new : Self :=
+    {| Bytes.value := [] |}.
+
+  Lemma new_eq (stack : Stack.t) :
+    {{
+      SimulateM.eval_f
+        links.mod.Impl_Bytes.run_new
+        stack 🌲
+      (
+        Output.Success new,
+        stack
+      )
+    }}.
+  Admitted.
+
+  Definition copy_from_slice (data : list u8) : Self :=
+    {| Bytes.value := data |}.
+
+  Lemma copy_from_slice_eq (ref_data : '& (list u8)) (stack : Stack.t) (data : list u8) :
+      CanRead.t stack data ref_data ->
+    {{
+      SimulateM.eval_f
+        (links.mod.Impl_Bytes.run_copy_from_slice ref_data)
+        stack 🌲
+      (
+        Output.Success (copy_from_slice data),
+        stack
+      )
+    }}.
+  Admitted.
+End Impl_Bytes.
