RocqOfRust/core/ops/simulate/deref.v
@@ -1,0 +1,33 @@
+Require Import simulate.RocqOfRust.
+Require Import core.ops.links.deref.
+
+(*
+pub trait Deref {
+    type Target: ?Sized;
+    fn deref(&self) -> &Self::Target;
+}
+*)
+Module Deref.
+  Class C (Self Target : Set) `{Link Self} `{Link Target} : Set := {
+    deref : RefStub.t Self Target;
+  }.
+
+  Module Eq.
+    Class t
+        {Self Target : Set} `{Link Self} `{Link Target}
+        `{!Deref.Run Self Target}
+        (I : C Self Target) :
+        Prop := {
+      deref (ref_self : '& Self) (stack : Stack.t) :
+        {{
+          SimulateM.eval_f
+            (Deref.run_deref ref_self)
+            stack 🌲
+          (
+            Output.Success (RefStub.apply ref_self I.(deref)),
+            stack
+          )
+        }};
+    }.
+  End Eq.
+End Deref.
