RocqOfRust/examples/default/examples/custom/links/fosdem.v
@@ -1,0 +1,81 @@
+Require Import links.RocqOfRust.
+Require Import examples.default.examples.custom.fosdem.
+
+(*
+struct Counter {
+  value: u64,
+}
+*)
+Module Counter.
+  Record t : Set := {
+    value : u64;
+  }.
+
+  Global Instance IsLink : Link t := {
+    Φ := Ty.path "fosdem::Counter";
+    φ x :=
+      Value.StructRecord "fosdem::Counter" [] [] [
+        ("value", φ x.(value))
+      ];
+  }.
+
+  Definition of_ty : OfTy.t (Ty.path "fosdem::Counter").
+  Proof. eapply OfTy.Make with (A := t); reflexivity. Defined.
+  Smpl Add apply of_ty : of_ty.
+
+  Lemma of_value_with value value' :
+    value' = φ value ->
+    Value.StructRecord "fosdem::Counter" [] [] [
+      ("value", value')
+    ] = φ (Build_t value).
+  Proof. now intros; subst. Qed.
+  Smpl Add apply of_value_with : of_value.
+
+  Definition of_value (value : u64) value' :
+    value' = φ value ->
+    OfValue.t (
+      Value.StructRecord "fosdem::Counter" [] [] [
+        ("value", value')
+      ]
+    ).
+  Proof.
+    intros.
+    eapply OfValue.Make with (A := t).
+    apply of_value_with; eassumption.
+  Defined.
+  Smpl Add eapply of_value : of_value.
+
+  Module SubPointer.
+    Definition get_value : SubPointer.Runner.t t
+      (Pointer.Index.StructRecord "fosdem::Counter" "value") :=
+    {|
+      SubPointer.Runner.projection x := Some x.(value);
+      SubPointer.Runner.injection x y := Some (x <| value := y |>);
+    |}.
+
+    Lemma get_value_is_valid :
+      SubPointer.Runner.Valid.t get_value.
+    Proof.
+      now constructor.
+    Qed.
+    Smpl Add apply get_value_is_valid : run_sub_pointer.
+  End SubPointer.
+End Counter.
+
+(* const MAX_VALUE: u64 = 1000 *)
+Instance run_MAX_VALUE :
+  Run.Trait value_MAX_VALUE [] [] [] ('* u64).
+Proof.
+  constructor.
+  run_symbolic.
+Defined.
+Global Opaque run_MAX_VALUE.
+
+(* impl Counter { fn increment(&mut self, amount: u64) } *)
+Instance run_increment (self : '&mut Counter.t) (amount : u64) :
+  Run.Trait Impl_fosdem_Counter.increment [] [] [φ self; φ amount] unit.
+Proof.
+  constructor.
+  run_symbolic.
+Defined.
+Global Opaque run_increment.
