RocqOfRust/links/RocqOfRust.v
@@ -3,3 +3,6 @@
 
 Require Export RocqOfRust.RocqOfRust.
 Require Export RocqOfRust.links.M.
+
+(* There is no export mode available at the moment. *)
+Global Opaque Z.add Z.sub Z.mul Z.div Z.modulo Z.pow.
